% Provides macros manipulating strings of tokens.
\RequirePackage{xstring}

% Store the jobname as a string with category 11 characters.
\edef\normaljobname{\expandafter\scantokens\expandafter{\jobname\noexpand}}
\StrBetween{\normaljobname}{hw-}{-q}[\homeworknumber]
\StrBehind{\normaljobname}{-q-}[\questionnumber]

\documentclass[
  coursecode={MTHE 474},
  assignmentname={Homework \homeworknumber},
  studentnumber=20053722,
  name={Bryan Hoang},
  draft,
  % final,
]{
  ltxanswer%
}

\usepackage{bch-style}

\renewcommand{\thepartno}{\roman{partno}}
\renewcommand{\thesubpart}{\alph{subpart}}
\renewcommand{\subpartlabel}{(\thesubpart)}

\begin{document}
  \begin{questions}
    \setcounter{question}{\questionnumber}
    \addtocounter{question}{-1}
    \question[20]\
    \begin{parts}
      \part\
      \begin{subparts}
        \subpart{}
        \begin{solution}
          \begin{proof}
            To prove the result, it is sufficient to show that \(\forall n \in \mathbb{Z}_{\ge0}\),
            \begin{align*}
              \frac{1}{n-1}H(X_{(n-1)+1}^{2(n-1)}|X^{n-1})                            &\ge \frac{1}{n}H(X_{n+1}^{2n}|X^{n}) \\
              \frac{1}{n-1}H(X_{n}^{2n-2}|X^{n-1}) - \frac{1}{n}H(X_{n+1}^{2n}|X^{n}) &\ge 0
            \end{align*}
            Thus, we have
            \begin{align*}
               &\phantomeq \frac{1}{n-1}H(X_{n}^{2n-2}|X^{n-1}) - \frac{1}{n}H(X_{n+1}^{2n}|X^{n})                                                                                                                  \\
               &= \frac{1}{n-1} H(X_{n}^{2n-2}|X^{n-1}) - \frac{1}{n} H(X_{n+1}^{2n}|X^{n})                                                                                                                         \\
               &= \frac{1}{n-1} \biggl[H(X_{1}^{2n-2}) - H(X^{n-1})\biggr] - \frac{1}{n} \biggl[H(X_{1}^{2n}) - H(X^{n})\biggr]                                                                                     \\
               &= \frac{1}{n-1} \biggl[\sum_{i=1}^{2n-2} H(X_{i}|X^{i-1}) - \sum_{i=1}^{n-1} H(X_{i}|X^{i-1})\biggr] - \frac{1}{n} \biggl[\sum_{i=1}^{2n} H(X_{i}|X^{i-1}) - \sum_{i=1}^{n} H(X_{i}|X^{i-1})\biggr] \\
               &= \frac{1}{n-1} \biggl[\sum_{i=n}^{2n-2} H(X_{i}|X^{i-1})\biggr] - \frac{1}{n} \biggl[\sum_{i=n+1}^{2n} H(X_{i}|X^{i-1})\biggr]                                                                     \\
              \intertext{By the stationarity of the source, we can re-index the first summation.}
               &= \frac{1}{n-1} \biggl[\sum_{i=n+1}^{2n-1} H(X_{i}|X_{2}^{i-1})\biggr] - \frac{1}{n} \biggl[\sum_{i=n+1}^{2n} H(X_{i}|X^{i-1})\biggr]                                                               \\
               &= \frac{1}{n(n-1)} \biggl[\sum_{i=n+1}^{2n-1} nH(X_{i}|X_{2}^{i-1}) - (n-1)H(X_{i}|X_{1}^{i-1}) \biggr] - \frac{1}{n} H(X_{2n}|X^{2n-1})                                                            \\
              \intertext{Since conditioning reduces entropy, we then have that}
               &\ge \frac{1}{n(n-1)} \biggl[\sum_{i=n+1}^{2n-1} nH(X_{i}|X_{1}^{i-1}) - (n-1)H(X_{i}|X_{1}^{i-1}) \biggr] - \frac{1}{n} H(X_{2n}|X^{2n-1})                                                          \\
               &= \frac{1}{n(n-1)} \biggl[\sum_{i=n+1}^{2n-1} H(X_{i}|X_{1}^{i-1})\biggr] - \frac{1}{n(n-1)}(n-1) H(X_{2n}|X^{2n-1})                                                                                \\
               &= \frac{1}{n(n-1)} \biggl[\sum_{i=n+1}^{2n-1} \underbrace{H(X_{i}|X_{1}^{i-1}) - H(X_{2n}|X^{2n-1})}_{D_{i}}\biggr]                                                                                 \\
               &\ge 0
            \end{align*}
            since the sequence of conditional entropies of a stationary source is nonincreasing, we have that \(D_{i} \ge 0,\ \forall i \in \{n+1, \dotsc, 2n-1\}\)
          \end{proof}
        \end{solution}

        \subpart{}
        \begin{solution}
          \begin{proof}
            \begin{proofpart} % 1
              Showing that \(H(X_{2n}|X^{2n-1}) \le \frac{1}{n}H(X_{n+1}^{2n}|X^{n})\).
              \begin{align*}
                 &\phantomeq \frac{1}{n}H(X_{n+1}^{2n}|X^{n}) - H(X_{2n}|X^{2n-1})                                                   \\
                 &= \frac{1}{n}\bigl[H(X^{2n}) - H(X^{n})\bigr] - H(X_{2n}|X^{2n-1})                                                 \\
                 &= \frac{1}{n}\biggl[\sum_{i=1}^{2n} H(X_{i}|X^{i-1}) - \sum_{i=1}^{n} H(X_{i}|X^{i-1})\biggr] - H(X_{2n}|X^{2n-1}) \\
                 &= \frac{1}{n}\biggl[\sum_{i=n+1}^{2n} H(X_{i}|X^{i-1})\biggr] - \frac{1}{n} \cdot n H(X_{2n}|X^{2n-1})             \\
                 &= \frac{1}{n}\biggl[\sum_{i=n+1}^{2n} \underbrace{H(X_{i}|X^{i-1}) - H(X_{2n}|X^{2n-1})}_{D_{i}}\biggr]            \\
                 &\ge 0
              \end{align*}
              since the sequence of conditional entropies of a stationary source is nonincreasing, we have that \(\forall i \in \{n+1,\dotsc,2n\}\),
              \begin{equation*}
                \begin{cases}
                  D_{i} \ge 0 &\text{if } i \neq 2n, \\
                  D_{i} = 0   &\text{if } i = 2n.
                \end{cases}
              \end{equation*}
            \end{proofpart}
            \begin{proofpart} % 2
              Showing that \(\frac{1}{n}H(X_{n+1}^{2n}|X^{n}) \le \frac{1}{n}H(X^{n})\).
              \begin{align*}
                 &\phantomeq \frac{1}{n}H(X^{n}) - \frac{1}{n}H(X_{n+1}^{2n}|X^{n})                                                                                    \\
                 &= \frac{1}{n} \Bigl[H(X^{n}) - \bigl(H(X^{2n}) - H(X^{n})\bigr) \Bigr]                                                                               \\
                 &= \frac{1}{n} \Bigl[H(X^{n}) - \bigl(H(X^{n}|X_{n+1}^{2n}) + H(X_{n+1}^{2n}) - H(X^{n})\bigr) \Bigr]                                                 \\
                 &= \frac{1}{n} \Bigl[H(X^{n}) - \bigl(H(X^{n}|X_{n+1}^{2n}) + H(X^{n}) - H(X^{n})\bigr) \Bigr]        & &\text{by stationarity}                       \\
                 &= \frac{1}{n} \bigl[H(X^{n}) - H(X^{n}|X_{n+1}^{2n})\bigr]                                                                                           \\
                 &\ge 0                                                                                                & &\because \text{conditioning reduces entropy}
              \end{align*}
            \end{proofpart}
          \end{proof}
        \end{solution}
      \end{subparts}
    \end{parts}
  \end{questions}
\end{document}
